examples/data_structures/graph/Graph.NodeSetSeq.fst
@@ -1,0 +1,43 @@
+module Graph.NodeSetSeq
+
+open FStar.Fin
+module SC = Seq.Complements
+module C = FStar.Classical
+open Graph.Base
+module S = FStar.Seq
+module E = Graph.Elementary
+
+let _in (s:S.seq 'a) = SC._in s
+let ( @^ ) (s:S.seq 'a) (i:_in s) : 'a = S.index s i
+
+let disjoint = SC.disjoint
+
+(* Not the same as union! *)
+let append (#n:nat)(n1 n2:nodesetseq n )
+ : Pure (nodesetseq n)
+ (requires (disjoint n1 n2))
+ (ensures (fun p' -> True))
+ =
+ E.lemma_mutually_exclusive_elementary_append n1 n2;
+ S.append n1 n2
+
+let lemma_disjoint_append (#n:nat) (n1 n2 n3: nodesetseq n)
+  : Lemma (requires (disjoint n1 n2) /\ (disjoint n1 n3) /\ (disjoint n2 n3))
+    (ensures (disjoint n1 n2 /\ disjoint (append n1 n2) n3))
+=   SC.lemma_disjoint_append n1 n2 n3
+
+let rec seq_to_nodesetseq_aux (#n:nat) (s:S.seq (fin n)) (n' : nodesetseq n)
+ : Pure (nodesetseq n) (requires (disjoint s n')) (ensures (fun p -> True)) (decreases (S.length s))
+ = match S.length s with
+ | 0 -> n'
+ | x -> let hd = S.head s in let tl = S.tail s in let hds = S.slice s 0 1 in
+   SC.lemma_disjoint_slice n' s 1 (S.length s); SC.lemma_disjoint_slice n' s 0 1;
+   let n'' = append hds n' in
+   if S.mem hd tl then seq_to_nodesetseq_aux tl n' 
+    else
+    (
+     SC.lemma_disjoint_append hds n' tl;
+     seq_to_nodesetseq_aux tl n''
+    )
+
+let seq_list_to_nodesetseq (#n:nat) (s:S.seq (fin n)) = seq_to_nodesetseq_aux s S.createEmpty
